app/src/main/dafny/vectorClock.dfy
@@ -1,40 +1,40 @@
-function Max(a: nat, b: nat): nat {
+function max(a: nat, b: nat): nat {
   if a >= b then a else b
 }
 
 datatype VectorClock = VectorClock(values: map<int, nat>)
 {
-  static function Empty(): VectorClock {
+  static function empty(): VectorClock {
     VectorClock(map[])
   }
 
-  function Inc(nr: int): VectorClock {
+  function inc(nr: int): VectorClock {
     VectorClock(values[nr := (if nr in values then values[nr] + 1 else 1)])
   }
 
-  predicate IsBefore(other: VectorClock) {
+  predicate isBefore(other: VectorClock) {
     values != other.values
     && (forall k | k in values :: k in other.values && values[k] <= other.values[k])
     && (forall k | k in other.values :: k in values ==> values[k] <= other.values[k])
   }
 
-  predicate IsConcurrent(other: VectorClock) {
-    !IsBefore(other) && !other.IsBefore(this)
+  predicate isConcurrent(other: VectorClock) {
+    !isBefore(other) && !other.isBefore(this)
   }
 
-  function Merge(other: VectorClock): (r: VectorClock)
+  function merge(other: VectorClock): (r: VectorClock)
     ensures forall k | k in values :: k in r.values
     ensures forall k | k in values :: r.values[k] >= values[k]
     ensures forall k | k in r.values :: k in values ==> r.values[k] >= values[k]
     ensures (forall k | k in values :: k in other.values && values[k] <= other.values[k]) ==> r.values == other.values
     ensures (forall k | k in other.values :: k in values && other.values[k] <= values[k]) ==> r.values == values
-    ensures !r.IsBefore(this)
-    ensures !r.IsBefore(other)
-    ensures IsBefore(other) ==> r.values == other.values
-    ensures other.IsBefore(this) ==> r.values == values
+    ensures !r.isBefore(this)
+    ensures !r.isBefore(other)
+    ensures isBefore(other) ==> r.values == other.values
+    ensures other.isBefore(this) ==> r.values == values
   {
     VectorClock( map k | k in values.Keys + other.values.Keys ::
-                   if k in values && k in other.values then Max(values[k], other.values[k])
+                   if k in values && k in other.values then max(values[k], other.values[k])
                    else if k in values then values[k] else other.values[k])
   }
 }
@@ -51,11 +51,11 @@ class VectorClockImpl {
 
   constructor()
     ensures Valid()
-    ensures clock == VectorClock.Empty()
+    ensures clock == VectorClock.empty()
     ensures values == map[]
   {
     values := map[];
-    clock := VectorClock.Empty();
+    clock := VectorClock.empty();
   }
 
   constructor FromMap(values: map<int, nat>)
@@ -71,9 +71,9 @@ class VectorClockImpl {
     requires Valid()
     ensures Valid()
     ensures fresh(r) && r.Valid()
-    ensures r.clock == clock.Inc(nr)
-    ensures this.clock.IsBefore(r.clock)
-    ensures !r.clock.IsBefore(this.clock)
+    ensures r.clock == clock.inc(nr)
+    ensures this.clock.isBefore(r.clock)
+    ensures !r.clock.isBefore(this.clock)
     ensures r.values == values[nr := (if nr in values then values[nr] + 1 else 1)]
   {
     if nr in values {
@@ -85,7 +85,7 @@ class VectorClockImpl {
 
   method isBefore(other: VectorClockImpl) returns (r: bool)
     requires Valid() && other.Valid()
-    ensures r == clock.IsBefore(other.clock)
+    ensures r == clock.isBefore(other.clock)
   {
     var keys := values.Keys;
     ghost var processed: set<int> := {};
@@ -124,7 +124,7 @@ class VectorClockImpl {
 
   method isConcurrent(other: VectorClockImpl) returns (r: bool)
     requires Valid() && other.Valid()
-    ensures r == clock.IsConcurrent(other.clock)
+    ensures r == clock.isConcurrent(other.clock)
   {
     var a := isBefore(other);
     var b := other.isBefore(this);
@@ -137,7 +137,7 @@ class VectorClockImpl {
     ensures (forall k | k in other.values :: k in values && other.values[k] <= values[k]) ==> r == values
   {
     map k | k in values.Keys + other.values.Keys ::
-      if k in values && k in other.values then Max(values[k], other.values[k])
+      if k in values && k in other.values then max(values[k], other.values[k])
       else if k in values then values[k] else other.values[k]
   }
 
@@ -145,14 +145,14 @@ class VectorClockImpl {
     requires Valid() && other.Valid()
     ensures Valid()
     ensures fresh(r) && r.Valid()
-    ensures r.clock == clock.Merge(other.clock)
+    ensures r.clock == clock.merge(other.clock)
     ensures r.values == MergedValues(other)
     ensures forall k | k in values :: r.values[k] >= values[k]
     ensures forall k | k in r.values :: k in values ==> r.values[k] >= values[k]
-    ensures !r.clock.IsBefore(this.clock)
-    ensures !r.clock.IsBefore(other.clock)
-    ensures clock.IsBefore(other.clock) ==> r.values == other.values
-    ensures other.clock.IsBefore(this.clock) ==> r.values == values
+    ensures !r.clock.isBefore(this.clock)
+    ensures !r.clock.isBefore(other.clock)
+    ensures clock.isBefore(other.clock) ==> r.values == other.values
+    ensures other.clock.isBefore(this.clock) ==> r.values == values
   {
     r := new VectorClockImpl.FromMap(MergedValues(other));
   }
