app/src/main/dafny/eventSet.dfy
@@ -1,0 +1,31 @@
+class Event{
+  constructor(){}
+}
+
+datatype EventSet=EventSet(events: set<Event>){
+  static function empty(): EventSet {
+    EventSet({})
+  }
+
+  method add() returns (r: EventSet)
+    ensures isBefore(r)
+    ensures fresh(r.events - events)
+  {
+    var e := new Event();
+    r := EventSet(events + {e});
+  }
+
+  function merge(other: EventSet): EventSet {
+    EventSet(events + other.events)
+  }
+
+  predicate isBefore(other: EventSet){
+    this!=other && forall e :: e in events ==> e in other.events
+  }
+
+  predicate isConcurrent(other: EventSet){
+    !this.isBefore(other) && !other.isBefore(this)
+  }
+}
+
+
