app/src/main/dafny/eventSetTests.dfy
@@ -1,0 +1,28 @@
+include "eventSet.dfy"
+include "vectorClock.dfy"
+
+method testBasics(){
+  var a:= EventSet.empty();
+  var b:=a.add();
+  var c:=a.add();
+  var d:=b.merge(c);
+  assert b.isConcurrent(c);
+  assert a.isBefore(b);
+  assert b.isBefore(d);
+  assert c.isBefore(d);
+}
+
+method testEquivalence(){
+  var a:=EventSet.empty();
+  var ac:=VectorClock.empty();
+
+  var b:=a.add();
+  var bc:=ac.inc(1);
+
+  var c:=a.add();
+  var cc:=ac.inc(2);
+
+  assert a.isBefore(b)== ac.isBefore(bc);
+  assert a.isBefore(c)== ac.isBefore(cc);
+  assert b.isBefore(c)== bc.isBefore(cc);
+}
