app/src/main/dafny/vectorClockTests.dfy
@@ -1,0 +1,8 @@
+include "vectorClock.dfy"
+method testConcurrentModification(){
+  var a:=VectorClock.empty();
+  var b:=a.inc(1);
+  var c:=a.inc(2);
+  var isConcurrent := b.isConcurrent(c);
+  assert isConcurrent;
+}
