app/validate.sh
@@ -1,0 +1,3 @@
+#!/bin/sh
+set -e
+dafny src/main/dafny/fileSystemTests.dfy
